

Practical 6

Lagrange and Newton interpolation

Lagrange Interpolation:

Find the for polynomial for the given function data:

Ques 2: (-1,5),(0,1),(1,1),(2,11)

```
In[25]:= xi = {-1, 0, 1, 2};
fi = {5, 1, 1, 11};
n = Length[xi];
For[k = 1, k ≤ n, k++,
  
$$L_k[x_] = \left( \prod_{j=1}^{k-1} \frac{x - xi[[j]]}{xi[[k]] - xi[[j]]} \right) * \left( \prod_{j=k+1}^n \frac{x - xi[[j]]}{xi[[k]] - xi[[j]]} \right);$$

  
$$P[x_] = \sum_{k=1}^n L_k[x] * fi[[k]];$$

Print["Lagrange polynomial P(x)=", P[x]]
Print["Simplified polynomial p(x)=", Simplify[P[x]]]
Print["Approximate value of x at x=1.5 is", P[1.5]]
```

Lagrange polynomial P(x)=

$$-\frac{5}{6} (1-x) (2-x) x + \frac{1}{2} (1-x) (2-x) (1+x) + \frac{1}{2} (2-x) x (1+x) + \frac{11}{6} (-1+x) x (1+x)$$

Simplified polynomial p(x)= $1 - 3x + 2x^2 + x^3$

Approximate value of x at x=1.5 is 4.375

Ques 2: $f(x)=\ln(x), x=1,2,3$

```
In[33]:= Clear[x, k, f, L, p]
xi = {1, 2, 3};
f[x_] := Log[x];
n = Length[xi];
For[k = 1, k ≤ n, k++,
  Lk[x_] =  $\left( \prod_{j=1}^{k-1} \frac{x - xi[[j]]}{xi[[k]] - xi[[j]]} \right) * \left( \prod_{j=k+1}^n \frac{x - xi[[j]]}{xi[[k]] - xi[[j]]} \right)$ ;
  P[x_] =  $\sum_{k=1}^n Lk[x] * N[f[xi[[k]]]]$ ;
Print["Lagrange polynomial P(x)=", P[x]]
Print["Simplified polynomial p(x)=", Simplify[P[x]]]
Print["Approximate value of x at x=1.5 is", P[1.5]]
Lagrange polynomial P(x)=0. + 0.693147 (3 - x) (-1 + x) + 0.549306 (-2 + x) (-1 + x)
Simplified polynomial p(x)=-0.980829 + 1.12467 x - 0.143841 x2
Approximate value of x at x=1.5 is0.382534
```

Newton Interpolation:

```

In[42]:= sum = 0;
points = {{3, 293}, {5, 508}, {6, 585}, {9, 764}};
n = Length[points]
y = points[[All, 1]]
f = points[[All, 2]]
dd[k_] :=
  Sum[
    (f[[i]] / Product[If[Equal[j, i], 1, (y[[i]] - y[[j]])], {j, 1, k}]), {i, 1, k}]
P[x_] =
  Sum[
    (dd[i] * Product[If[i ≤ j, 1, x - y[[j]]], {j, 1, i - 1}]), {i, 1, n}]
Simplify[P[x]]
Evaluate[P[2.5]]

```

Out[44]= 4

Out[45]= {3, 5, 6, 9}

Out[46]= {293, 508, 585, 764}

Out[48]= $293 + \frac{215}{2} (-3 + x) - \frac{61}{6} (-5 + x) (-3 + x) + \frac{35}{36} (-6 + x) (-5 + x) (-3 + x)$

Out[49]= $\frac{1}{36} (-9702 + 9003 x - 856 x^2 + 35 x^3)$

Out[50]= 222.288